format-version: 1.2
ontology: http://www.semanticweb.org/ontologies/2012/9/Ontology1350918386851.owl/http://www.semanticweb.org/ontologies/2012/9/Ontology1350918386851.owl-relaxed

[Term]
id: BFO:0000003
name: occurrent
namespace: FlyBase development CV
def: "An entity that has temporal parts and that happens, unfolds or develops through time. Sometimes also called perdurants." [BFOC:ANON]
disjoint_from: http://www.semanticweb.org/ontologies/2010/5/Ontology1275387730635.owl:NRTF0000015 ! event
created_by: djs93
creation_date: 2009-10-01T05:56:28Z

[Term]
id: FBcv:0000025
name: lethal - all die during pharate adult stage
def: "A phenotype of a population that is the death of all animals in that population during the pharate adult stage." [FBC:DOS]
is_a: FBcv:0002005 ! lethal - all die during P-stage
is_a: FBcv:0002036 ! majority die during pharate adult stage
relationship: RO:0002092 FBdv:00006011 ! happens_during pharate adult stage

[Term]
id: FBcv:0000026
name: lethal - all die before end of prepupal stage
def: "A phenotype of a population that is the death of all animals in that population at some stage or stages before the end of the prepupal stage." [FBC:DOS]
is_a: FBcv:0000027 ! lethal - all die before end of pupal stage
relationship: BFO:0000060 FBdv:00005349 ! precedes pupal stage

[Term]
id: FBcv:0000027
name: lethal - all die before end of pupal stage
def: "A phenotype of a population that is the death of all animals in that population at some stage or stages before the end of the pupal stage." [FBC:DOS]
is_a: FBcv:0002000 ! lethal - all die before end of P-stage
relationship: BFO:0000060 FBdv:00006011 ! precedes pharate adult stage

[Term]
id: FBcv:0000347
name: phenotype

[Term]
id: FBcv:0000351
name: lethal
def: "A phenotype of a population that is the death of all animals in that population at some stage or stages prior to becoming a mature adult, where mature is defined as after adult stage A3 (FBdv:00006012)." [FBC:DOS, FBC:KM]
is_a: FBcv:0002019 ! some die before mature adult stage
relationship: BFO:0000060 FBdv:00007026 ! precedes mature adult stage

[Term]
id: FBcv:0002000
name: lethal - all die before end of P-stage
def: "A phenotype of a population that is the death of all animals in that population at some stage or stages prior to eclosion from the pupal case (the end of the P-stage)." [FBC:DOS]
comment: As the P-Stage and the 'pharate adult stage' have the same end,  there is no need for a seprate term for 'lethal - all die before end of pharate adult stage.
synonym: "lethal - all die before end of pharate adult stage" EXACT []
is_a: FBcv:0000351 ! lethal
relationship: BFO:0000060 FBdv:00005370 ! precedes adult stage A1

[Term]
id: FBcv:0002001
name: lethal - all die before end of first instar larval stage
def: "A phenotype of a population that is the death of all animals in that population at some stage or stages before the end of the first instar larval stage." [FBC:DOS]
is_a: FBcv:0002003 ! lethal - all die before end of second instar larval stage
relationship: BFO:0000060 FBdv:00005338 ! precedes second instar larval stage

[Term]
id: FBcv:0002002
name: lethal - all die before end of larval stage
def: "A phenotype of a population that is the death of all animals in that population at some stage or stages before the end of the larval stage." [FBC:DOS]
comment: As the larval stage and third instar larval stage have the same end,  there is no need for a separate term for 'lethal - all die before end of third instar larval stage'.
synonym: "lethal - all die before end of third instar larval stage" EXACT []
is_a: FBcv:0000026 ! lethal - all die before end of prepupal stage
relationship: BFO:0000060 FBdv:00005342 ! precedes prepupal stage

[Term]
id: FBcv:0002003
name: lethal - all die before end of second instar larval stage
def: "A phenotype of a population that is the death of all animals in that population at some stage or stages before the end of the second instar larval stage." [FBC:DOS]
is_a: FBcv:0002002 ! lethal - all die before end of larval stage
relationship: BFO:0000060 FBdv:00005339 ! precedes third instar larval stage

[Term]
id: FBcv:0002005
name: lethal - all die during P-stage
def: "A phenotype of a population that is the death of all animals in that population during the P-stage." [FBC:DOS]
is_a: FBcv:0002000 ! lethal - all die before end of P-stage
is_a: FBcv:0002010 ! majority die during P-stage
relationship: RO:0002092 FBdv:00007001 ! happens_during P-stage

[Term]
id: FBcv:0002006
name: lethal - all die during first instar stage
def: "A phenotype of a population that is the death of all animals in that population during the first instar larval stage." [FBC:DOS]
is_a: FBcv:0002001 ! lethal - all die before end of first instar larval stage
is_a: FBcv:0002007 ! lethal - all die during larval stage
is_a: FBcv:0002011 ! majority die during first instar larval stage
relationship: RO:0002092 FBdv:00005337 ! happens_during first instar larval stage

[Term]
id: FBcv:0002007
name: lethal - all die during larval stage
def: "A phenotype of a population that is the death of all animals in that population during the larval stage." [FBC:DOS]
is_a: FBcv:0002002 ! lethal - all die before end of larval stage
is_a: FBcv:0002012 ! majority die during larval stage
relationship: RO:0002092 FBdv:00005336 ! happens_during larval stage

[Term]
id: FBcv:0002008
name: lethal - all die during second instar stage
def: "A phenotype of a population that is the death of all animals in that population during the second instar larval stage." [FBC:DOS]
is_a: FBcv:0002003 ! lethal - all die before end of second instar larval stage
is_a: FBcv:0002007 ! lethal - all die during larval stage
is_a: FBcv:0002013 ! majority die during second instar larval stage
relationship: RO:0002092 FBdv:00005338 ! happens_during second instar larval stage

[Term]
id: FBcv:0002009
name: lethal - all die during third instar stage
def: "A phenotype of a population that is the death of all animals in that population during the third instar larval stage." [FBC:DOS]
is_a: FBcv:0002007 ! lethal - all die during larval stage
is_a: FBcv:0002014 ! majority die during third instar larval stage
relationship: RO:0002092 FBdv:00005339 ! happens_during third instar larval stage

[Term]
id: FBcv:0002010
name: majority die during P-stage
def: "A phenotype of a population that is the death of the majority of animals in that population during the P-stage." []
is_a: FBcv:0002020 ! some die during P-stage
relationship: RO:0002092 FBdv:00007001 ! happens_during P-stage

[Term]
id: FBcv:0002011
name: majority die during first instar larval stage
def: "A phenotype of a population that is the death of the majority of animals in that population during the \nfirst instar larval stage." [FBC:DOS]
is_a: FBcv:0002012 ! majority die during larval stage
is_a: FBcv:0002021 ! some die during first instar larval stage
relationship: RO:0002092 FBdv:00005337 ! happens_during first instar larval stage

[Term]
id: FBcv:0002012
name: majority die during larval stage
def: "A phenotype of a population that is the death of the majority of animals in that population during the \nlarval stage." []
is_a: FBcv:0002023 ! some die during larval stage
relationship: RO:0002092 FBdv:00005336 ! happens_during larval stage

[Term]
id: FBcv:0002013
name: majority die during second instar larval stage
def: "A phenotype of a population that is the death of the majority of animals in that population during the \nsecond instar larval stage." [FBC:DOS]
is_a: FBcv:0002012 ! majority die during larval stage
is_a: FBcv:0002022 ! some die during second instar larval stage
relationship: RO:0002092 FBdv:00005338 ! happens_during second instar larval stage

[Term]
id: FBcv:0002014
name: majority die during third instar larval stage
def: "A phenotype of a population that is the death of the majority of animals in that population during the \nthird instar larval stage." [FBC:DOS]
is_a: FBcv:0002012 ! majority die during larval stage
is_a: FBcv:0002024 ! some die during third instar larval stage
relationship: RO:0002092 FBdv:00005339 ! happens_during third instar larval stage

[Term]
id: FBcv:0002015
name: partially lethal
def: "A phenotype of a population that is the death of some significant proportion of animals in that population prior to becoming a mature adult, where mature is defined as after adult stage A3 (FBdv:00006012)." [FBC:DOS, FBC:KM]
is_a: FBcv:0002019 ! some die before mature adult stage
relationship: BFO:0000060 FBdv:00007026 ! precedes mature adult stage

[Term]
id: FBcv:0002016
name: partially lethal - majority die
def: "A phenotype of a population that is the death a majority of animals in that population prior to becoming a mature adult, where mature is defined as after adult stage A3 (FBdv:00006012)." [FBC:DOS, FBC:NB]
is_a: FBcv:0002015 ! partially lethal
relationship: BFO:0000060 FBdv:00007026 ! precedes mature adult stage

[Term]
id: FBcv:0002017
name: partially lethal - majority live
def: "A phenotype of a population that is the death of some significant proportion of animals in that population, but less that half, prior to becoming a mature adult, where mature is defined as after adult stage A3 (FBdv:00006012)." [FBC:DOS]
is_a: FBcv:0002015 ! partially lethal
relationship: BFO:0000060 FBdv:00007026 ! precedes mature adult stage

[Term]
id: FBcv:0002019
name: some die before mature adult stage
def: "A phenotype of a population that is the death a significant proportion of animals in that population prior to becoming a mature adult, where mature is defined as after adult stage A3 (FBdv:00006012)." [FBC:DOS]
is_a: BFO:0000003 ! occurrent
is_a: scratch:0008217 ! mortality
relationship: BFO:0000060 FBdv:00007026 ! precedes mature adult stage

[Term]
id: FBcv:0002020
name: some die during P-stage
def: "A phenotype of a population that is the death a significant proportion of animals in that population during the P-stage." [FBC:DOS]
is_a: FBcv:0002019 ! some die before mature adult stage
relationship: RO:0002092 FBdv:00007001 ! happens_during P-stage

[Term]
id: FBcv:0002021
name: some die during first instar larval stage
def: "A phenotype of a population that is the death a significant proportion of animals in that population during the first instar larval stage." [FBC:DOS]
is_a: FBcv:0002023 ! some die during larval stage
relationship: RO:0002092 FBdv:00005337 ! happens_during first instar larval stage

[Term]
id: FBcv:0002022
name: some die during second instar larval stage
def: "A phenotype of a population that is the death a significant proportion of animals in that population during the second instar larval stage." [FBC:DOS]
is_a: FBcv:0002023 ! some die during larval stage
relationship: RO:0002092 FBdv:00005338 ! happens_during second instar larval stage

[Term]
id: FBcv:0002023
name: some die during larval stage
def: "A phenotype of a population that is the death a significant proportion of animals in that population during the larval stage." [FBC:DOS]
is_a: FBcv:0002019 ! some die before mature adult stage
relationship: RO:0002092 FBdv:00005336 ! happens_during larval stage

[Term]
id: FBcv:0002024
name: some die during third instar larval stage
def: "A phenotype of a population that is the death a significant proportion of animals in that population during the third instar larval stage." [FBC:DOS]
is_a: FBcv:0002023 ! some die during larval stage
relationship: RO:0002092 FBdv:00005339 ! happens_during third instar larval stage

[Term]
id: FBcv:0002030
name: lethal - all die during pupal stage
def: "A phenotype of a population that is the death of all animals in that population during the pupal stage." [FBC:DOS]
is_a: FBcv:0000027 ! lethal - all die before end of pupal stage
is_a: FBcv:0002005 ! lethal - all die during P-stage
is_a: FBcv:0002034 ! majority die during pupal stage
relationship: RO:0002092 FBdv:00005349 ! happens_during pupal stage

[Term]
id: FBcv:0002031
name: lethal - all die during prepupal stage
def: "A phenotype of a population that is the death of all animals in that population during the prepupal stage." [FBC:DOS]
is_a: FBcv:0000026 ! lethal - all die before end of prepupal stage
is_a: FBcv:0002005 ! lethal - all die during P-stage
is_a: FBcv:0002035 ! majority die during prepupal stage
relationship: RO:0002092 FBdv:00005342 ! happens_during prepupal stage

[Term]
id: FBcv:0002032
name: lethal - all die before end of embryonic stage
def: "A phenotype of a population that is the death of all animals in that population at some stage or stages before the end of the embryonic stage." [FBC:DOS]
is_a: FBcv:0002001 ! lethal - all die before end of first instar larval stage
relationship: BFO:0000060 FBdv:00005337 ! precedes first instar larval stage

[Term]
id: FBcv:0002033
name: lethal - all die during embryonic stage
def: "A phenotype of a population that is the death of all animals in that population during the embryonic stage." [FBC:DOS]
is_a: FBcv:0002032 ! lethal - all die before end of embryonic stage
is_a: FBcv:0002037 ! majority die during embryonic stage
relationship: RO:0002092 FBdv:00005289 ! happens_during embryonic stage

[Term]
id: FBcv:0002034
name: majority die during pupal stage
def: "A phenotype of a population that is the death of the majority of animals in that population during the \npupal stage." [FBC:DOS]
is_a: FBcv:0002010 ! majority die during P-stage
is_a: FBcv:0002039 ! some die during pupal stage
relationship: RO:0002092 FBdv:00005349 ! happens_during pupal stage

[Term]
id: FBcv:0002035
name: majority die during prepupal stage
def: "A phenotype of a population that is the death of the majority of animals in that population during the \nprepual stage." [FBC:DOS]
is_a: FBcv:0002010 ! majority die during P-stage
is_a: FBcv:0002040 ! some die during prepupal stage
relationship: RO:0002092 FBdv:00005342 ! happens_during prepupal stage

[Term]
id: FBcv:0002036
name: majority die during pharate adult stage
def: "A phenotype of a population that is the death of the majority of animals in that population during the \npharate adult stage." [FBC:DOS]
is_a: FBcv:0002010 ! majority die during P-stage
is_a: FBcv:0002038 ! some die during pharate adult stage
relationship: RO:0002092 FBdv:00006011 ! happens_during pharate adult stage

[Term]
id: FBcv:0002037
name: majority die during embryonic stage
def: "A phenotype of a population that is the death of the majority of animals in that population during the embryonic stage." [FBC:DOS]
comment: This term is agnostic about whether any survive to adulthood.
is_a: FBcv:0002041 ! some die during embryonic stage
relationship: RO:0002092 FBdv:00005289 ! happens_during embryonic stage

[Term]
id: FBcv:0002038
name: some die during pharate adult stage
def: "A phenotype of a population that is the death a significant proportion of animals in that population during the pharate adult stage." [FBC:DOS]
is_a: FBcv:0002020 ! some die during P-stage
relationship: RO:0002092 FBdv:00006011 ! happens_during pharate adult stage

[Term]
id: FBcv:0002039
name: some die during pupal stage
def: "A phenotype of a population that is the death a significant proportion of animals in that population during the pupal stage." [FBC:DOS]
is_a: FBcv:0002020 ! some die during P-stage
relationship: RO:0002092 FBdv:00005349 ! happens_during pupal stage

[Term]
id: FBcv:0002040
name: some die during prepupal stage
def: "A phenotype of a population that is the death a significant proportion of animals in that population during the prepual stage." [FBC:DOS]
is_a: FBcv:0002020 ! some die during P-stage
relationship: RO:0002092 FBdv:00005342 ! happens_during prepupal stage

[Term]
id: FBcv:0002041
name: some die during embryonic stage
def: "A phenotype of a population that is the death a significant proportion of animals in that population during the embryonic stage." [FBC:DOS]
is_a: FBcv:0002019 ! some die before mature adult stage
relationship: RO:0002092 FBdv:00005289 ! happens_during embryonic stage

[Term]
id: FBcv:0002042
name: lethal - all die during immature adult stage
def: "A phenotype of a population that is the death of all animals in that population as immature adults (after eclosion but before the end of adult stage A3 (FBdv:00006012))." [FBC:DOS]
is_a: FBcv:0000351 ! lethal
is_a: FBcv:0002050 ! majority die during immature adult stage
relationship: RO:0002092 FBdv:00006012 ! happens_during adult stage A3

[Term]
id: FBcv:0002050
name: majority die during immature adult stage
def: "A phenotype of a population that is the death of the majority of animals in that population as immature adults (after eclosion but before the end of adult stage A3 (FBdv:00006012))." [FBC:DOS]
is_a: FBcv:0002051 ! some die during immature adult stage
relationship: RO:0002092 FBdv:00007025 ! happens_during immature adult stage

[Term]
id: FBcv:0002051
name: some die during immature adult stage
def: "A phenotype of a population that is the death of some significant number of animals in that population as immature adults (after eclosion but before the end of adult stage A3 (FBdv:00006012))." [FBC:DOS]
is_a: FBcv:0002019 ! some die before mature adult stage
relationship: RO:0002092 FBdv:00007025 ! happens_during immature adult stage

[Term]
id: FBdv:00005259
name: developmental stage
namespace: FlyBase development CV
alt_id: FBdv:00007010
def: "A temporal subdivision of a developmental process." [FBC:DOS]
is_a: BFO:0000003 ! occurrent
created_by: djs93
creation_date: 2009-10-01T05:56:56Z

[Term]
id: FBdv:00005289
name: embryonic stage
namespace: FlyBase development CV
def: "The stage of the Drosophila life-cycle from fertilisation to hatching." [FBC:DOS]
comment: Temporal ordering number - 20.
is_a: FBdv:00007012 ! life stage
relationship: ends_at_start_of FBdv:00005336 ! larval stage
relationship: ends_at_start_of FBdv:00005337 ! first instar larval stage

[Term]
id: FBdv:00005336
name: larval stage
namespace: FlyBase development CV
def: "The stage of the Drosophila life-cycle from hatching to the beginning of puparium formation." [FBC:DOS]
comment: Temporal ordering number - 400.
is_a: FBdv:00007012 ! life stage
relationship: ends_at_start_of FBdv:00005342 ! prepupal stage
relationship: ends_at_start_of FBdv:00007001 ! P-stage
relationship: starts_at_end_of FBdv:00005289 ! embryonic stage

[Term]
id: FBdv:00005337
name: first instar larval stage
namespace: FlyBase development CV
def: "The first larval instar begins at hatching and ends at the first larval molt. Anterior spiracles are not yet present; posterior spiracles have two openings each. Salivary glands are very small and all cells are uniform in size. Mouth hooks typically have one tooth. Duration at 25 degrees C: approximately 25 hours (24-49 hours after egg laying; 0-25 hours after hatching)." [FlyBase:FBrf0007733]
comment: Temporal ordering number - 410.
synonym: "first instar larva" EXACT []
synonym: "L1" EXACT []
is_a: FBdv:00007012 ! life stage
relationship: BFO:0000050 FBdv:00005336 ! part_of larval stage
relationship: ends_at_start_of FBdv:00005338 ! second instar larval stage
relationship: starts_at_end_of FBdv:00005289 ! embryonic stage

[Term]
id: FBdv:00005338
name: second instar larval stage
namespace: FlyBase development CV
def: "The second larval instar begins at the first larval molt and ends at the second larval molt. Larvae are actively feeding and crawling in the food. Distinct anterior spiracles are present as enlargements at the end of the tracheal trunk, but not open to the outside; posterior spiracles have three openings each, and four groups of small unbranched hairs. The salivary glands extend to the first abdominal segment, and have cells that are uniform in size. Mouth hooks typically have two or three teeth. Duration at 25 degrees C: approximately 23 hours (49-72 hours after egg laying; 25-48 hours after hatching)." [FlyBase:FBrf0007733]
comment: Temporal ordering number - 420.
synonym: "L2" EXACT []
synonym: "second instar larva" EXACT []
is_a: FBdv:00007012 ! life stage
relationship: BFO:0000050 FBdv:00005336 ! part_of larval stage
relationship: ends_at_start_of FBdv:00005339 ! third instar larval stage
relationship: starts_at_end_of FBdv:00005337 ! first instar larval stage

[Term]
id: FBdv:00005339
name: third instar larval stage
namespace: FlyBase development CV
def: "The third larval instar begins at the second larval molt and ends at puparium formation. Anterior spiracles are open to the outside; posterior spiracles have three openings each, and four groups of large branched hairs. The salivary glands extend to the second abdominal segment, with cells larger in the posterior than in the anterior of the gland. Mouth hooks typically have 9-12 teeth. About 24 hours before pupariation (at 25 degree C), larvae stop feeding and climb away from their food. Duration at 25 degrees C: approximately 48 hours (72-120 hours after egg laying; 48-96 hours after hatching)." [FlyBase:FBrf0007733]
comment: Temporal ordering number - 430.
synonym: "L3" EXACT []
synonym: "third instar larva" RELATED []
is_a: FBdv:00007012 ! life stage
relationship: BFO:0000050 FBdv:00005336 ! part_of larval stage
relationship: ends_at_start_of FBdv:00005342 ! prepupal stage
relationship: ends_at_start_of FBdv:00007001 ! P-stage
relationship: starts_at_end_of FBdv:00005338 ! second instar larval stage

[Term]
id: FBdv:00005342
name: prepupal stage
namespace: FlyBase development CV
def: "The prepupal stage begins at puparium formation and ends when larval/pupal apolysis is complete, as indicated by the completion of imaginal head sac eversion and the expulsion of the oral armature of the larva. Duration at 25 degrees C: approximately 12 hours. (120-132.2 hours after egg laying; 0-12.2 hours after puparium formation)." [FlyBase:FBrf0036849, FlyBase:FBrf0048355]
comment: Temporal ordering number - 500.
is_a: FBdv:00007012 ! life stage
relationship: BFO:0000050 FBdv:00007001 ! part_of P-stage
relationship: ends_at_start_of FBdv:00005349 ! pupal stage
relationship: starts_at_end_of FBdv:00005336 ! larval stage
relationship: starts_at_end_of FBdv:00005339 ! third instar larval stage

[Term]
id: FBdv:00005349
name: pupal stage
namespace: FlyBase development CV
def: "The pupal stage starts once larval/pupal apolysis is complete as indicated by the expulsion of the larval armature. Early in this stage, the legs and wings reach full extension along the abdomen. The stage ends when the pupal cuticle separates from the underlying epidermis (pupal/adult apolysis), and the eye cup becomes yellow at its periphery. Duration at 25 degrees C: approximately 32 hours. (132.2-164.3 hours after egg laying; 12.2-44.3 hours after puparium formation)." [FlyBase:FBrf0036849, FlyBase:FBrf0048355]
comment: Temporal ordering number - 570. DISAMBIGUATION: In Drosophila lab vernacular, the term 'pupal stage' is often used to refer to the entire period from formation of the puparium to eclosion. However, this does not correspond to the standard usage of 'pupal stage' for Cyclorrhaphous flies (for discussion see: FBrf0087128). Briefly: formation of the puparium (hardening of the larval cuticle) marks the beginning of the pre-pupal stage. The pupal stage begins following pupal/larval apolysis - detachment of the larval epidermis from the puparium. In Drosophila, the outward sign of the completion of apolysis is the eversion of the head and expulsion of the larval mouthparts (FBrf0036849). We use P-stage to refer to the stage from pupariation to eclosion, and restrict pupal stage to its standard usage.
synonym: "phanerocephalic pupa" EXACT [FlyBase:FBrf0036849]
is_a: FBdv:00007012 ! life stage
relationship: BFO:0000050 FBdv:00007001 ! part_of P-stage
relationship: ends_at_start_of FBdv:00006011 ! pharate adult stage
relationship: starts_at_end_of FBdv:00005342 ! prepupal stage

[Term]
id: FBdv:00005369
name: adult stage
namespace: FlyBase development CV
def: "The stage of the Drosophila life-cycle from eclosion to death." [FBC:DOS]
comment: Temporal ordering number - 770.
is_a: FBdv:00007012 ! life stage
relationship: starts_at_end_of FBdv:00006011 ! pharate adult stage
relationship: starts_at_end_of FBdv:00007001 ! P-stage

[Term]
id: FBdv:00005370
name: adult stage A1
namespace: FlyBase development CV
alt_id: FBdv:00005373
def: "Newly eclosed adult stage. Animal free of pupal case. Runs rapidly to find site for wing expansion. Wings are folded back and black against a very pale abdomen." [FlyBase:FBrf0049147]
comment: Temporal ordering number - 785.  The time at which eclosed flies settle down for wing expansion can vary greatly.  If they fail to find a suitable site then expansion can be delayed by several hours.
synonym: "adult stage I" RELATED []
is_a: FBdv:00005259 ! developmental stage
relationship: BFO:0000050 FBdv:00007025 ! part_of immature adult stage
relationship: ends_at_start_of FBdv:00005371 ! adult stage A2
relationship: starts_at_end_of FBdv:00006011 ! pharate adult stage
relationship: starts_at_end_of FBdv:00007001 ! P-stage

[Term]
id: FBdv:00005371
name: adult stage A2
namespace: FlyBase development CV
alt_id: FBdv:00005374
def: "Stage, shortly after eclosion, during which the wings expand. During wing expansion, the abdomen pulsates and the hind legs stroke the wings vigorously for several minutes at a time. The stage ends when the wings are folded down over the abdomen, which has become broader and shorter, and the wing cuticle has lost its folds.  The stage lasts around 15 minutes at 25'C." [FlyBase:FBrf0049147]
comment: Temporal ordering number - 790.
synonym: "adult stage II" RELATED []
is_a: FBdv:00005259 ! developmental stage
relationship: BFO:0000050 FBdv:00007025 ! part_of immature adult stage
relationship: ends_at_start_of FBdv:00006012 ! adult stage A3
relationship: starts_at_end_of FBdv:00005370 ! adult stage A1

[Term]
id: FBdv:00006011
name: pharate adult stage
namespace: FlyBase development CV
def: "The developing adult after pupal-adult apolysis , i.e.- from stage P8 (when yellow eye color first becomes visible through the pupal case), to eclosion. Duration at 25 degrees C: approximately 55.7 hours (164.3-220 hours after egg laying; 44.3-100 hours after puparium formation)." [FlyBase:FBrf0036849, FlyBase:FBrf0048355, FlyBase:FBrf0049147]
comment: Temporal ordering number - 625.
is_a: FBdv:00007012 ! life stage
relationship: BFO:0000050 FBdv:00007001 ! part_of P-stage
relationship: ends_at_start_of FBdv:00005369 ! adult stage
relationship: ends_at_start_of FBdv:00005370 ! adult stage A1
relationship: ends_at_start_of FBdv:00007025 ! immature adult stage
relationship: starts_at_end_of FBdv:00005349 ! pupal stage

[Term]
id: FBdv:00006012
name: adult stage A3
namespace: FlyBase development CV
alt_id: FBdv:00005375
def: "Adult stage immediately after wing expansion, during which tanning of the cuticle is completed.  This stage lasts approximately 45 minutes at 25'C." [FlyBase:FBrf0049147]
comment: Temporal ordering number - 800.
synonym: "adult stage III" RELATED []
is_a: FBdv:00005259 ! developmental stage
relationship: BFO:0000050 FBdv:00007025 ! part_of immature adult stage
relationship: ends_at_start_of FBdv:00007026 ! mature adult stage
relationship: starts_at_end_of FBdv:00005371 ! adult stage A2

[Term]
id: FBdv:00007001
name: P-stage
namespace: FlyBase development CV
def: "The stage of the Drosophila life-cycle from the formation of the puparium (beginning of the prepupal stage) to eclosion." [FBC:DOS]
comment: Temporal ordering number - 490. DISAMBIGUATION: In Drosophila lab vernacular, the term 'pupal stage' is often used to refer to the entire period from formation of the puparium to eclosion. However, this does not correspond to the standard usage of 'pupal stage' for Cyclorrhaphous flies (for discussion see: FBrf0087128). Briefly: formation of the puparium (hardening of the larval cuticle) marks the beginning of the pre-pupal stage. The pupal stage begins following pupal/larval apolysis - detachment of the larval epidermis from the puparium. In Drosophila, the outward sign of the completion of apolysis is the eversion of the head an expulsion of the larval mouthparts (FBrf0036849). We use P-stage to refer to the stage from pupariation to eclosion, and restrict pupal stage to its standard usage.
synonym: "metamorphosis" BROAD []
synonym: "pupal stage" RELATED []
is_a: FBdv:00007012 ! life stage
relationship: ends_at_start_of FBdv:00005369 ! adult stage
relationship: ends_at_start_of FBdv:00005370 ! adult stage A1
relationship: ends_at_start_of FBdv:00007025 ! immature adult stage
relationship: starts_at_end_of FBdv:00005336 ! larval stage
relationship: starts_at_end_of FBdv:00005339 ! third instar larval stage
created_by: david
creation_date: 2008-06-05T04:51:40Z

[Term]
id: FBdv:00007012
name: life stage
namespace: FlyBase development CV
def: "A temporal subdivision of a Drosophila life, delimited by major transitions in the circumstances of the organism, such as: fertilisation; hatching; pupal ecdysis; eclosion." [FBC:DOS]
synonym: "life cycle stage" RELATED []
is_a: FBdv:00005259 ! developmental stage
created_by: djs93
creation_date: 2009-10-01T05:59:22Z

[Term]
id: FBdv:00007025
name: immature adult stage
namespace: FlyBase development CV
def: "The developmental stage that lasts from eclosion of the adult from the pupal case until tanning is complete (the end of adult stage A3)." [FBC:DOS]
comment: Temporal ordering number - 782.
is_a: FBdv:00007012 ! life stage
relationship: ends_at_start_of FBdv:00007026 ! mature adult stage
relationship: starts_at_end_of FBdv:00006011 ! pharate adult stage
relationship: starts_at_end_of FBdv:00007001 ! P-stage
created_by: djs93
creation_date: 2013-01-08T20:06:59Z

[Term]
id: FBdv:00007026
name: mature adult stage
namespace: FlyBase development CV
def: "Life stage from the end of adult stage A3, when tanning is complete, to death." [FBC:DOS]
is_a: FBdv:00007012 ! life stage
relationship: starts_at_end_of FBdv:00006012 ! adult stage A3
relationship: starts_at_end_of FBdv:00007025 ! immature adult stage
created_by: djs93
creation_date: 2013-01-10T13:03:54Z

[Term]
id: http://www.semanticweb.org/ontologies/2010/5/Ontology1275387730635.owl:NRTF0000015
name: event
comment: time dimension = 0.  An event is an instant.
is_a: owl:Thing

[Term]
id: scratch:0008217
name: mortality
is_a: FBcv:0000347 ! phenotype

[Typedef]
id: BFO:0000050
name: part_of
namespace: FlyBase development CV
synonym: "part_of" EXACT []
xref: BFO:0000050
xref: OBO_REL:part_of
is_transitive: true
is_a: RO:0002092 ! happens_during

[Typedef]
id: BFO:0000060
name: precedes
comment: X precedes Y iff: end(X) before_or_simultaneous_with start(Y)
synonym: "ends_before" EXACT []
domain: BFO:0000003 ! occurrent
range: BFO:0000003 ! occurrent
is_transitive: true
is_a: RO:0002089 ! starts_before
inverse_of: preceded_by ! preceded_by
holds_over_chain: RO:0002092 BFO:0000060 ! happens_during precedes
holds_over_chain: RO:0002093 BFO:0000060 ! ends_during precedes

[Typedef]
id: RO:0002081
name: before_or_simultaneous_with
comment: Primitive instance level timing relation between events
synonym: "<=" EXACT []
domain: http://www.semanticweb.org/ontologies/2010/5/Ontology1275387730635.owl:NRTF0000015 ! event
range: http://www.semanticweb.org/ontologies/2010/5/Ontology1275387730635.owl:NRTF0000015 ! event

[Typedef]
id: RO:0002082
name: simultaneous_with
comment: t1 simultaneous_with t2 iff:=  t1 before_or_simultaneous_with t2  and not (t1 before t2)
domain: http://www.semanticweb.org/ontologies/2010/5/Ontology1275387730635.owl:NRTF0000015 ! event
range: http://www.semanticweb.org/ontologies/2010/5/Ontology1275387730635.owl:NRTF0000015 ! event
is_transitive: true
is_a: RO:0002081 ! before_or_simultaneous_with

[Typedef]
id: RO:0002083
name: before
comment: t1 before t2 iff:=  t1 before_or_simulataneous_with t2  and not (t1 simultaeous_with t2)
domain: http://www.semanticweb.org/ontologies/2010/5/Ontology1275387730635.owl:NRTF0000015 ! event
range: http://www.semanticweb.org/ontologies/2010/5/Ontology1275387730635.owl:NRTF0000015 ! event
is_transitive: true
is_a: RO:0002081 ! before_or_simultaneous_with

[Typedef]
id: RO:0002084
name: during_which_ends
comment: Perviously used http://purl.obolibrary.org/obo/RO_0002122 - but this seems to have been dropped from ro-edit.owl at some point.  No re-use under this ID AFAIK, but leaving note here in case we run in to clashes down the line.
inverse_of: RO:0002093 ! ends_during

[Typedef]
id: RO:0002085
name: encompasses
comment: Previously had ID  http://purl.obolibrary.org/obo/RO_0002124 in test files in sandpit - but this seems to have been dropped from ro-edit.owl at some point.  No re-use under this ID AFAIK, but leaving note here in case we run in to clashes down the line.  Official ID now chosen from DOS ID range.
is_transitive: true
is_a: RO:0002084 ! during_which_ends
is_a: RO:0002088 ! during_which_starts
inverse_of: RO:0002092 ! happens_during

[Typedef]
id: RO:0002086
name: ends_after
comment: X ends_after Y iff: end(Y) before_or_simultaneous_with end(X)
domain: BFO:0000003 ! occurrent
range: BFO:0000003 ! occurrent
is_transitive: true
holds_over_chain: RO:0002093 preceded_by ! ends_during preceded_by

[Typedef]
id: RO:0002088
name: during_which_starts
comment: Previously had ID  http://purl.obolibrary.org/obo/RO_0002123 in test files in sandpit - but this seems to have been dropped from ro-edit.owl at some point.  No re-use under this ID AFAIK, but leaving note here in case we run in to clashes down the line.  Official ID now chosen from DOS ID range.
inverse_of: RO:0002091 ! starts_during

[Typedef]
id: RO:0002089
name: starts_before
domain: BFO:0000003 ! occurrent
range: BFO:0000003 ! occurrent
is_transitive: true
holds_over_chain: RO:0002091 BFO:0000060 ! starts_during precedes

[Typedef]
id: RO:0002091
name: starts_during
comment: X starts_during Y iff: (start(Y) before_or_simultaneous_with start(X)) AND (start(X) before_or_simultaneous_with end(Y))
domain: BFO:0000003 ! occurrent
range: BFO:0000003 ! occurrent

[Typedef]
id: RO:0002092
name: happens_during
comment: X happens_during Y iff: (start(Y) before_or_simultaneous_with start(X)) AND (end(X) before_or_simultaneous_with end(Y))
is_transitive: true
is_a: RO:0002091 ! starts_during
is_a: RO:0002093 ! ends_during

[Typedef]
id: RO:0002093
name: ends_during
comment: X ends_during Y iff: ((start(Y) before_or_simultaneous_with end(X)) AND end(X) before_or_simultaneous_with end(Y). 
domain: BFO:0000003 ! occurrent
range: BFO:0000003 ! occurrent

[Typedef]
id: ends_at_start_of
name: immediately_precedes
namespace: FlyBase development CV
comment: X immediately_precedes_Y iff: end(X) simultaneous_with start(Y)
synonym: "ends_at_start_of" EXACT []
xref: RO:0002090
domain: BFO:0000003 ! occurrent
range: BFO:0000003 ! occurrent
is_a: BFO:0000060 ! precedes

[Typedef]
id: preceded_by
name: preceded_by
namespace: FlyBase development CV
comment: X preceded_by Y iff: end(Y) before_or_simultaneous_with start(X)
synonym: "proceeds" EXACT []
synonym: "starts_after" EXACT []
xref: BFO:0000062
xref: OBO_REL:preceded_by
domain: BFO:0000003 ! occurrent
range: BFO:0000003 ! occurrent
is_transitive: true
is_a: RO:0002086 ! ends_after
holds_over_chain: RO:0002091 preceded_by ! starts_during preceded_by
holds_over_chain: RO:0002092 preceded_by ! happens_during preceded_by
created_by: djs93
creation_date: 2009-10-09T10:00:53Z

[Typedef]
id: starts_at_end_of
name: immediately_preceded_by
namespace: FlyBase development CV
comment: X immediately_preceded_by Y iff: end(X) simultaneous_with start(Y)
synonym: "starts_at_end_of" EXACT []
xref: RO:0002087
domain: BFO:0000003 ! occurrent
range: BFO:0000003 ! occurrent
is_a: preceded_by ! preceded_by
inverse_of: ends_at_start_of ! immediately_precedes

